progress

lean4/Crypto/Structure.lean
@@ -1,49 +1,50 @@
 import Lean
 import Crypto.Util
+
 open Lean Elab Tactic Meta
+
+namespace Crypto
 
 /-- `isIn e l` tests whether `e` is definitionally equal to an expression in `l`. -/
 def isIn (e : Expr) (es : Array Expr) : MetaM Bool :=
 es.foldrM (init := false) λ e' b => do b || (← isDefEq e e')
 
--- /-- `getDefEq e l` tries to find the first expression `f` in `l` definitionally equal to `e`. -/
--- def getDefEq (e : Expr) (es : Array Expr) : MetaM Bool :=
--- es.findM? λ e' => _do if (← isDefEq e e') then _ else
+-- #check getMVarType
+-- #check assignExprMVar
+-- #check liftMetaMAtMain
+-- #check getMainGoal
+-- #check withMainContext
+-- #check evalGeneralize
+-- #check Parser.Tactic.generalize
 
-
-
--- def AddToContext (lctx : LocalContext) (h : Name) (t : Expr) : MetaM (LocalContext × FVarId) := do
---   let nm ← mkFreshFVarId
---   let new_lctx := lctx.addDecl (mkLocalDeclEx 0 nm h t BinderInfo.default)
---   return (new_lctx, nm)
-
-#check getMVarType
-#check assignExprMVar
-#check liftMetaMAtMain
-#check getMainGoal
-#check withMainContext
-#check evalGeneralize
-#check Parser.Tactic.generalize
-
--- #check Parser.Tactic.have
+/- the data we record for each field -/
 structure FieldData where
 (decl : LocalDecl)
 (fvar : Expr)
 (type : Expr)
 (depends : NameSet)
 (isProp : Bool)
+deriving Inhabited
 
+/- additionally an expression that gives us the translation to another field -/
 structure FieldMapping extends FieldData where
 (tgt : Option Expr)
+
+structure Context where
+(target : Array FieldData)
+
+structure State where
+(mapping : Array FieldMapping)
 
 open Std.Format
 
 instance : ToFormat NameSet :=
-⟨λ x => fmt x.toList⟩
+⟨λ x => format x.toList⟩
 
 instance : ToFormat FieldData :=
-⟨λ ⟨a, b, c, d, e⟩ => group (nest 1 (fmt "⟨"  ++ fmt a ++ fmt "," ++ line ++ fmt b ++ fmt "," ++ line
-++ fmt c ++ fmt "," ++ line ++ fmt d ++ fmt "," ++ line ++ fmt e ++ fmt "⟩"))⟩
+⟨λ ⟨a, b, c, d, e⟩ => group (nest 1 (format "⟨"  ++ format a ++ format "," ++ line ++ format b ++
+format "," ++ line ++ format c ++ format "," ++ line ++ format d ++ format "," ++ line ++ format e
+++ format "⟩"))⟩
 
 namespace FieldData
 
@@ -55,15 +56,63 @@ def toFieldMapping (fields : FieldData) : FieldMapping :=
 
 end FieldData
 
-namespace Meta
+namespace FieldMapping
+def update (field : FieldMapping) (newM : Option Expr) : FieldMapping :=
+if field.tgt.isNone then { field with tgt := newM } else field
+
+def updateM (field : FieldMapping) (tac : MetaM (Option Expr)) : MetaM FieldMapping :=
+if field.tgt.isNone then do
+  let tgt ← tac
+  return { field with tgt := tgt }
+else
+  return field
+
+end FieldMapping
 
 def ppFieldData (x : FieldData) : MetaM Format :=
-do return group (nest 1 (fmt "⟨"  ++
-fmt x.name ++ fmt "," ++ line ++
-fmt (← ppExpr x.fvar) ++ fmt "," ++ line ++
-fmt (← ppExpr x.type) ++ fmt "," ++ line ++
-fmt (← x.depends.toList.mapM λ e => ppExpr (mkFVar e)) ++ fmt "," ++ line ++
-fmt x.isProp ++ fmt "⟩"))
+do return group (nest 1 (format "⟨"  ++
+format x.name ++ format "," ++ line ++
+format (← ppExpr x.fvar) ++ format "," ++ line ++
+format (← ppExpr x.type) ++ format "," ++ line ++
+format (← x.depends.toList.mapM λ e => ppExpr (mkFVar e)) ++ format "," ++ line ++
+format x.isProp ++ format "⟩"))
+
+/-- make a field mapping with no connections. -/
+def mkState (fields1 : Array FieldData) : State :=
+{ mapping := fields1.map λ info => { toFieldData := info, tgt := none } }
+
+namespace State
+
+def done (st : State) : Bool :=
+st.mapping.all (·.tgt.isSome)
+
+def update (st : State) (f : FieldData → Option Expr) : State :=
+{ mapping := st.mapping.map λ info => info.update (f info.toFieldData) }
+
+def updateM (st : State) (f : FieldData → MetaM (Option Expr)) : MetaM State := do
+  let fieldMapping ← st.mapping.mapM λ info => info.updateM (f info.toFieldData)
+  return { mapping := fieldMapping }
+
+def getDataMapping (st : State) : Array (Expr × Expr) :=
+st.mapping.filterMap λ map => match map.tgt with
+  | none => none
+  | some e => if map.isProp then none else some (map.fvar, e)
+
+def getMapping (st : State) : Array (Expr × Expr) :=
+st.mapping.filterMap λ map => match map.tgt with
+  | none => none
+  | some e => some (map.fvar, e)
+
+def missing (st : State) : Array FieldData :=
+st.mapping.filterMap λ info => if info.tgt.isNone then some info.toFieldData else none
+
+def missingData (st : State) : Array FieldData :=
+st.mapping.filterMap λ info =>
+  if info.tgt.isNone && !info.isProp then some info.toFieldData else none
+
+end State
+
+namespace Meta
 
 def AddFieldsToContext (mvarId : MVarId) (nm : Name) (us : List Level) (args : Array Expr) :
   MetaM (MVarId × MVarId × Array FieldData) := do
@@ -84,35 +133,20 @@ def AddFieldsToContext (mvarId : MVarId) (nm : Name) (us : List Level) (args : A
   let types ← fieldExprs.mapM inferType
   let depends := types.map λ tp => tp.ListFvarIds
   let fieldData := ldecls.zipWith5 FieldData.mk fieldExprs types depends axiom_fields
-  -- IO.println f!"field data: {← fieldData.mapM ppFieldData}"
   return (mvarId, m2, fieldData)
 
--- for testing
-def trivialMapping (lctx : LocalContext) (fields1 fields2 : Array FieldData) :
-  MetaM $ Array (Expr × Expr) × Array FieldMapping := do
-  let fieldMapping :=
-    fields1.map λ info => FieldMapping.mk info $
-      if info.isProp then none else
-      fields2.findSome! λ info' => if info.name == info'.name then some info'.fvar else none
-  let mapping := fieldMapping.filterMap λ map =>
-    if map.tgt.isSome then some (map.fvar, map.tgt.get!) else none
-  let dataFields := fields1.filter λ info => !info.isProp
-  let map1 ← dataFields.map (·.fvar)
-  let map2 ← dataFields.map λ info => fields2.findSome! λ info' =>
-    if info.name == info'.name then some info'.fvar else none
-  -- let map2 := map2.map λ info? => info?.getD arbitrary
-  --(info.fvar.fvarId!.updateSuffix λ s => "h2" ++ s) |>.toExpr
-  return (mapping, fieldMapping)
+/-- map the data fields to data fields of the same name. -/
+def trivialMapping (lctx : LocalContext) (st : State) (ctx : Context) : State :=
+st.update $ λ info =>
+  if info.isProp then none else
+    ctx.target.findSome? λ info' => if info.name == info'.name then some info'.fvar else none
 
-def mkFieldMapping (fields1 fields2 : Array FieldData) :
-  MetaM $ Array (Expr × Expr) := do
-  let dataFields := fields1.filter λ info => !info.isProp
-  let map1 ← dataFields.map (·.fvar)
-  let map2 ← dataFields.map λ info => fields2.findSome! λ info' =>
-    if info.name == info'.name then some info'.fvar else none
-  -- let map2 := map2.map λ info? => info?.getD arbitrary
-  --(info.fvar.fvarId!.updateSuffix λ s => "h2" ++ s) |>.toExpr
-  return (map1.zip map2)
+/-- map the data fields to data fields with the same type, if a unique such data field exists. -/
+def uniqueMapping (lctx : LocalContext) (st : State) (ctx : Context) : MetaM State :=
+st.updateM $ λ info => if info.isProp then return none else do
+  let sources ← st.mapping.filterM λ info' => isDefEq info.type info'.type
+  let targets ← ctx.target.filterM λ info' => isDefEq info.type info'.type
+  return (if sources.size = 1 ∧ targets.size = 1 then some (targets.get! 0).fvar else none)
 
 -- todo
 def allMappings (fields1 fields2 : Array FieldData) : MetaM $ List $ List (FVarId × Expr) := do
@@ -121,152 +155,129 @@ def allMappings (fields1 fields2 : Array FieldData) : MetaM $ List $ List (FVarI
  throwError "todo"
 
 /-- Find which axioms in fields1 also occur in fields2 under the renaming `mapping`. -/
-def matchingAxioms (fields1 fields2 : Array FieldData) (mapping : Array (Expr × Expr)) :
-  MetaM $ Array FieldData := do
-  let propFields := fields1.filter λ info => info.isProp
-  let types2 : Array Expr := fields2.filterMap λ info => if info.isProp then info.type else none
-  let same ← propFields.filterM λ info => isIn (info.type.instantiateFVars mapping) types2
-  return same
+def matchingAxioms (st : State) (ctx : Context) : MetaM State := do
+  -- let propFields := fields1.filter λ info => info.isProp
+  let types2 : Array Expr := ctx.target.filterMap λ info => if info.isProp then info.type else none
+  let fieldMapping ←
+    st.mapping.mapM λ info => info.updateM $ do {
+      -- types2.findM? λ e' => do b || (← isDefEq e e')
 
--- /-- Find which axioms in fields1 also occur in fields2 under the renaming `mapping`. -/
--- def matchingAxioms2 (fields1 : Array FieldMapping) (fields2 : Array FieldData)
---   (mapping : Array (Expr × Expr)) :
---   MetaM $ Array FieldMapping := do
---   let propFields := fields1.filter λ info => info.isProp
---   let types2 : Array Expr := fields2.filterMap λ info => if info.isProp then info.type else none
---   let same ← propFields.mapM λ info => isIn (info.type.instantiateFVars mapping) types2
---   return same
+--todo:
+      if (← isIn (info.type.instantiateFVars st.getDataMapping) types2) then
+        return (some arbitrary) else return none }
+  return { mapping := fieldMapping }
 
-def mkSimpContext (simpOnly := false) : MetaM Simp.Context := do
-  return {
-    config      := {}
+/-- some copy-pasted simp code -/
+def getPropHyps : MetaM (Array FVarId) := do
+  let mut result := #[]
+  for localDecl in (← getLCtx) do
+    unless localDecl.isAuxDecl do
+      if (← isProp localDecl.type) then
+        result := result.push localDecl.fvarId
+  return result
+
+/-- some mostly copy-pasted simp code -/
+def mkSimpContext (simpOnly := false) (starArg := true) : MetaM Simp.Context := do
+  let ctx : Simp.Context :=
+  { config      := {}
     simpLemmas  := if simpOnly then {} else (← getSimpLemmas)
-    congrLemmas := (← getCongrLemmas)
-  }
+    congrLemmas := (← getCongrLemmas) }
+  if !starArg then
+    return ctx
+  else
+    let hs ← getPropHyps
+    let mut ctx := ctx
+    for h in hs do
+      let localDecl ← getLocalDecl h
+      let fvarId := localDecl.fvarId
+      let proof  := localDecl.toExpr
+      let id     ← mkFreshUserName `h
+      let simpLemmas ← ctx.simpLemmas.add #[] proof (name? := id)
+      ctx := { ctx with simpLemmas }
+    return ctx
 
 /-- The tactic we use to automatically prove axioms. -/
 def currentAutomation (mvarId : MVarId) : MetaM Unit := do
-match (← simpTarget mvarId (← mkSimpContext false)) with -- does this work?
-| some x => return () --IO.println "failure!"
-| none => return ()  -- IO.println "success!"
+let newgoal ← simpTarget mvarId (← mkSimpContext false)
 
-#print elabSimpConfig
-#print replaceMainGoal
-
---return () -- tidy >> (done <|> tactic.interactive.finish [] none)
+-- match (← simpTarget mvarId (← mkSimpContext false)) with
+-- | some x => IO.println "failure!"
+-- | none => IO.println "success!"
 
 /-- Tries to prove `e` in the local context, returns tt if successful. -/
-def tryToProve (mvarId : MVarId) (e : Expr) : MetaM Bool := withoutModifyingState do
+def tryToProve (mvarId : MVarId) (tac : MVarId → MetaM Unit) (e : Expr) : MetaM (Option Expr) :=
+withoutModifyingState do
   let (fvar, mvarId, m2) ← assertm mvarId `h e
   try
-    currentAutomation m2
+    tac m2
     -- IO.println s!"is assigned: {← isExprMVarAssigned m2}"
-    let some e ← getExprMVarAssignment? m2 | return false
+    let some e ← getExprMVarAssignment? m2 | return none
     let e ← instantiateMVars e
-    if (← e.hasExprMVar) then return false else return true
+    if (← e.hasExprMVar) then return none else return some e
   catch err =>
-    return false
-
+    return none
 
 /-- Tests whether nm1 is a subclass of nm1. Currently the data fields must have the same Name for
 this tactic to work. -/
-def isSubclass (mvarId : MVarId) (nm1 nm2 : Name) (show_state := false) :
-  MetaM (MVarId × MVarId × MVarId) := do
+def isSubclass (mvarId : MVarId) (nm1 nm2 : Name) (show_state := false) (trace := true) :
+  MetaM (MVarId × MVarId × MVarId × State) := do
   let u := mkLevelParam `u
   let (M, mvarId) ← asserti mvarId `M (mkSort (mkLevelSucc u)) (mkConst `PUnit [mkLevelSucc u])
   let (mvarId, m1, fields1) ← AddFieldsToContext mvarId nm1 [u] #[mkFVar M]
   let (mvarId, m2, fields2) ← AddFieldsToContext mvarId nm2 [u] #[mkFVar M]
   -- let mapping := fields1.map (·.toFieldMapping)
   withMVarContext mvarId do
-  let (mapping, fieldMapping) ← trivialMapping (← getLCtx) fields1 fields2
-  -- IO.println f!"map 1: {← map1.mapM Meta.ppExpr}"
-  -- IO.println f!"map 2: {← map2.mapM Meta.ppExpr}"
-  let matching ← matchingAxioms fields1 fields2 mapping
-  let matchingUniqs := matching.map λ info => info.fvar.fvarId!
-  let todo := fields1.filter λ info => info.isProp && !matchingUniqs.contains info.fvar.fvarId!
-  if todo.isEmpty then
-    IO.println s!"{nm1} is a trivial subclass of {nm2}: {nm2} has all the fields that {nm1} has."
-  else do
-    -- trace $ todo.map λ info => info.fvar.local_pp_name,
-    -- let cannot_prove ← todo.filterM λ info => bnot <$> try_to_prove (info.type.instantiate_locals mapping),
-    let cannotProve ← todo.filterM λ info =>
-      not <$> tryToProve mvarId (info.type.instantiateFVars mapping)
-    -- trace $ cannot_prove.map λ info => info.fvar.local_pp_name,
-    if cannotProve.isEmpty then
-    IO.println s!"{nm1} is a subclass of {nm2}: {nm2} has all the data fields of {nm1}, and all the axioms of {nm1} can be proven from the axioms of {nm2}."
-    else
-    IO.println s!"Cannot prove the following axioms of {nm1} from the axioms of {nm2}:
-    {← cannotProve.mapM λ info : FieldData => ppExpr info.fvar}."
-  return (mvarId, m1, m2)
+  let st := mkState fields1
+  let ctx : Context := ⟨fields2⟩
+  let st ← uniqueMapping (← getLCtx) st ctx
+  let st ← trivialMapping (← getLCtx) st ctx
+  let st ← matchingAxioms st ctx
+  let st ← st.updateM λ info =>
+    tryToProve mvarId currentAutomation (info.type.instantiateFVars st.getDataMapping)
+  if st.done then
+    IO.println s!"{nm1} is a subclass of {nm2}"
+  else
+    IO.println s!"Cannot construct the following fields of {nm1} from {nm2}:
+    {← st.missing.mapM λ info : FieldData => ppExpr info.fvar}."
+  return (mvarId, m1, m2, st)
 
 end Meta
-open Meta
 
--- def strucTacticM (mvarId : MVarId) : MetaM (MVarId × MVarId × Array FieldData) := do
---   let nm := `comm_monoid1
---   let e ← getEnv
---   let d ← e.find? nm
---   let tt ← isStructureLike e nm
---   let u := mkLevelParam `u
---   let (M, mvarId) ← asserti mvarId `M (mkSort (mkLevelSucc u)) (mkConst `PUnit [mkLevelSucc u])
---   let eStr ← mkAppN (mkConst nm [u]) #[mkFVar M]
---   let (h, mvarId, m2) ← assertm mvarId `h eStr
---   let l ← cases mvarId h
---   let info := l.get! 0
---   let mvarId := info.mvarId
---   withMVarContext mvarId do
---   let lctx ← getLCtx
---   let fieldExprs := info.fields
---   let fields := fieldExprs.map Expr.fvarId!
---   let ldecls := fields.map λ e => lctx.fvarIdToDecl.find! e
---   let axiom_fields ← fieldExprs.mapM isProof
---   let types ← fieldExprs.mapM inferType
---   let depends := types.map λ tp => tp.ListFvarIds
---   let fieldData := ldecls.zipWith5 FieldData.mk fieldExprs types depends axiom_fields
---   IO.println f!"field data: {← fieldData.mapM ppFieldData}"
---   return (mvarId, m2, fieldData)
-
-
-syntax (name := assert) "assert " ident (" : " term) (" := " term)? : tactic
-@[tactic assert] def evalAssert : Tactic := fun stx =>
+syntax (name := guardHyp) "guardHyp " (" : " term)? : tactic
+@[tactic guardHyp] def evalGuardHyp : Lean.Elab.Tactic.Tactic := fun stx =>
   match stx with
-  | `(tactic| assert $h : $ty $[:= $val]?) => do
-    withMainContext do
-      let mvarId ← getMainGoal
-      let eTy ← elabTerm ty none
-      match val with
-      | none   => do
-        let (h, m1, m2) ← assertm mvarId h.getId eTy
-        let l ← getUnsolvedGoals
-        setGoals (m1::m2::l)
-      | some v => do
-        let eV ← elabTerm v eTy
-        let (hs, m) ← assertHypotheses mvarId #[⟨h.getId, eTy, eV⟩]
-        let l ← getUnsolvedGoals
-        setGoals (m::l)
+  | `(tactic| guardHyp $[: $ty]?) => do
+    return ()
   | _ => throwUnsupportedSyntax
 
--- syntax (name := struc) "struc" : tactic
--- @[tactic «struc»] def evalStruc : Tactic := fun stx => do
---   match stx with
---   | `(tactic| struc) => withMainContext do
---     let mvarId ← getMainGoal
---     let (m1, m2, data) ← strucTacticM mvarId
---     let l ← getUnsolvedGoals
---     setGoals (m1::m2::l)
---   | _ => throwUnsupportedSyntax
+def isSubclassTac (nm1 nm2 : Name) : TacticM Unit := withMainContext do
+let mvarId ← getMainGoal
+let (mvarId, m1, m2, result) ← Meta.isSubclass mvarId nm1 nm2
+let l ← getUnsolvedGoals
+setGoals (mvarId::m1::m2::l)
 
 syntax (name := isSubclass) "isSubclass " ident ident : tactic
-@[tactic «isSubclass»] def evalIsSubclass : Tactic := fun stx => do
+syntax (name := isSubclassE) "isSubclass! " ident ident : tactic
+@[tactic «isSubclass»] def evalIsSubclass : Tactic := fun stx =>
   match stx with
-  | `(tactic| isSubclass $nm1 $nm2) => withMainContext do
-    let mvarId ← getMainGoal
-    let (mvarId, m1, m2) ← Meta.isSubclass mvarId nm1.getId nm2.getId
-    let l ← getUnsolvedGoals
-    setGoals (mvarId::m1::m2::l)
+  | `(tactic| isSubclass $nm1 $nm2) => withoutModifyingState $ isSubclassTac nm1.getId nm2.getId
+  | _ => throwUnsupportedSyntax
+@[tactic «isSubclassE»] def evalIsSubclassE : Tactic := fun stx =>
+  match stx with
+  | `(tactic| isSubclass! $nm1 $nm2) => isSubclassTac nm1.getId nm2.getId
   | _ => throwUnsupportedSyntax
 
-/-! We define two notions of commutative monoids, the first is right-unital and the second is both left-unital and right-unital. -/
+
+end Crypto
+
+/-!
+We define some notions of commutative monoids,
+* the first is right-unital
+* the second is right-unital, and then has a superfluous axiom `1 * 1 = 1`
+* the third is both left-unital and right-unital.
+* the fourth is with a implicit unit
+* the fifth is denoted additively
+-/
 
 class comm_monoid1 (M : Type _) :=
 (mul : M → M → M)
@@ -280,31 +291,40 @@ class comm_monoid2 (M : Type _) :=
 (mul : M → M → M)
 (mul_one : ∀ x, mul x one = x)
 (one_mul_one : mul one one = one)
+(mul_assoc : ∀ x y z, mul (mul x y) z = mul x (mul y z))
+(mul_comm : ∀ x y, mul x y = mul y x)
+
+class comm_monoid3 (M : Type _) :=
+(one : M)
+(mul : M → M → M)
+(mul_one : ∀ x, mul x one = x)
 (one_mul : ∀ x, mul one x = x)
 (mul_assoc : ∀ x y z, mul (mul x y) z = mul x (mul y z))
 (mul_comm : ∀ x y, mul x y = mul y x)
 
+class comm_monoid4 (M : Type _) :=
+(mul : M → M → M)
+(mul_assoc : ∀ x y z, mul (mul x y) z = mul x (mul y z))
+(mul_comm : ∀ x y, mul x y = mul y x)
+(exists_one : ∃ one, ∀ x, mul x one = x)
 
--- example : Unit := by
---   struc
---   exact ()
---   admit
+class comm_monoid5 (M : Type _) :=
+(add : M → M → M)
+(add_assoc : ∀ x y z, add (add x y) z = add x (add y z))
+(add_comm : ∀ x y, add x y = add y x)
+(zero : M)
+(add_zero : ∀ x, add x zero = x)
 
 example : Unit := by
-  isSubclass comm_monoid1 comm_monoid2
-  isSubclass comm_monoid2 comm_monoid1
+  isSubclass comm_monoid1 comm_monoid2 -- subclass
+  isSubclass comm_monoid2 comm_monoid1 -- subclass
+  isSubclass comm_monoid1 comm_monoid3 -- subclass
+  isSubclass comm_monoid3 comm_monoid1 -- missing: one_mul
+  isSubclass comm_monoid1 comm_monoid5 -- subclass
+  isSubclass comm_monoid5 comm_monoid1 -- subclass
+  isSubclass comm_monoid4 comm_monoid1 -- missing: exists_one
+  isSubclass comm_monoid1 comm_monoid4 -- missing: one, mul_one
   exact ()
-  admit
-  admit
-  admit
-  admit
-
--- #eval is_subclass `comm_monoid1 `comm_monoid2
-/- Output: comm_monoid1 is a trivial subclass of comm_monoid2: comm_monoid2 has all the fields that comm_monoid1 has. -/
-
--- #eval is_subclass `comm_monoid2 `comm_monoid1
-/- Output: comm_monoid2 is a subclass of comm_monoid1: comm_monoid1 has all the data fields of comm_monoid2, and all the axioms of comm_monoid2 can be proven from the axioms of comm_monoid1. -/
-
 
 /-! As a sanity check: we cannot prove commutativity on an arbitrary monoid. -/
 
@@ -314,6 +334,23 @@ class my_monoid (M : Type _) :=
 (one : M)
 (mul_one : ∀ x, mul x one = x)
 
--- #eval is_subclass `comm_monoid1 `my_monoid
-/- Output: Cannot prove the following axioms of comm_monoid1 from the axioms of my_monoid:
-[mul_comm]. -/
+example : Unit := by
+  isSubclass my_monoid comm_monoid1 -- subclass
+  isSubclass comm_monoid1 my_monoid -- missing (as expected): mul_comm
+  exact ()
+
+/-! If two data fields have the same type, we try to get the one with the same name.
+In the future we could look at which choice will make more axioms overlap. -/
+
+class my_almost_ring (M : Type _) :=
+(add : M → M → M)
+(mul : M → M → M)
+(mul_assoc : ∀ x y z, mul (mul x y) z = mul x (mul y z))
+(mul_comm : ∀ x y, mul x y = mul y x)
+(one : M)
+(mul_one : ∀ x, mul x one = x)
+
+example : Unit := by
+  isSubclass comm_monoid1 my_almost_ring -- subclass
+  isSubclass my_almost_ring comm_monoid1 -- missing (as expected): add
+  exact ()
